stuff

CacheCoherence.v
@@ -1,558 +1,493 @@
 Require Import CpdtTactics.
 Load Useful.
 
-Definition Time := nat.
-Definition State := nat.
+Module Classical.
+  Hypothesis dec: forall P: Prop, P \/ ~ P.
+End Classical.
 
-Inductive Channel := pc | cp.
-Definition Mesg := (State * State)%type.
+Module Type Mesg.
+  Parameter mesg: Type.
+End Mesg.
 
-Inductive enq : Channel -> Mesg -> Time -> Prop :=
-  enq_intro : forall s m t, enq s m t.
+Module Type FifoHighLevel (mesg: Mesg).
+  Import mesg.
 
-Inductive deq : Channel -> Mesg -> Time -> Prop :=
-  deq_intro : forall s m t, deq s m t.
+  Inductive enq : mesg -> nat -> Prop :=
+    enq_intro : forall m t, enq m t.
+
+  Inductive deq : mesg -> nat -> Prop :=
+    deq_intro : forall m t, deq m t.
+
+  Axiom uniqueEnq1: forall {m n t1 t2}, enq m t1 -> enq n t2 -> m = n -> t1 = t2.
+
+  Axiom uniqueEnq2: forall {m n t1 t2}, enq m t1 -> enq n t2 -> t1 = t2 -> m = n.
+
+  Axiom uniqueDeq1: forall {m n t1 t2}, deq m t1 -> deq n t2 -> m = n -> t1 = t2.
+
+  Axiom uniqueDeq2: forall {m n t1 t2}, deq m t1 -> deq n t2 -> t1 = t2 -> m = n.
+
+  Axiom deqImpEnq: forall {m t}, deq m t -> exists t', t' <= t /\ enq m t'.
+
+  Axiom fifo1: 
+      forall {m te td}, enq m te -> deq m td -> forall {m' te' td'}, enq m' te' -> deq m' td' -> te' < te -> td' < td.
+
+  Axiom fifo2:
+      forall {m te td}, enq m te -> deq m td -> forall {m' te' td'}, enq m' te' -> deq m' td' -> td' < td -> te' < te.
+
+  Theorem fifo1' {m te td} (enqM: enq m te) (deqM: deq m td) {m' te' td'} (enqM': enq m' te') (deqM': deq m' td'): te' <= te -> td' <= td.
+  Proof.
+    intro te'LeTe.
+    assert (cases: te' = te \/ te' < te) by crush.
+    destruct cases as [te'EqTe | te'LtTe].
+    assert (m' = m) by (apply (uniqueEnq2 enqM' enqM); crush).
+    assert (td' = td) by (apply (uniqueDeq1 deqM' deqM); crush).
+    crush.
+    assert (td' < td) by (apply (fifo1 enqM deqM enqM' deqM'); crush).
+    crush.
+  Qed.
+
+  Theorem fifo2':
+    forall {m te td}, enq m te -> deq m td -> forall {m' te' td'}, enq m' te' -> deq m' td' -> td' <= td -> te' <= te.
+  Proof.
+    intros.
+    assert (cases: td' = td \/ td' < td) by crush.
+    destruct cases as [td'EqTd | td'LtTd].
+    assert (m = m') by (apply (uniqueDeq2 H0 H2); crush).
+    assert (te' = te) by (apply (uniqueEnq1 H1 H); crush).
+    crush.
+    assert (te' < te) by (apply (fifo2 H H0 H1 H2); crush).
+    crush.
+  Qed.
+
+  Theorem enq0First {m t} (enq0: enq m 0) (deqT: deq m t) t' (lt: t' < t) m' (deqM': deq m' t'): False.
+  Proof.
+    pose proof (deqImpEnq deqM') as exEnq.
+    destruct exEnq as [t'' rest].
+    destruct rest as [leEnq enqM'].
+    pose proof (fifo2 enq0 deqT enqM' deqM' lt).
+    crush.
+  Qed.
+End FifoHighLevel.
 
 Inductive Point := p | c.
+Definition State := nat.
 
-Definition sendm pt m t :=
-  match pt with
-    | p => enq pc m t
-    | c => enq cp m t
-  end.
+Module RespMesg <: Mesg.
+  Definition mesg := (State * State)%type.
+End RespMesg.
 
-Definition recvm pt m t :=
-  match pt with
-    | p => deq cp m t
-    | c => deq pc m t
-  end.
+Module Type Resp (pc: FifoHighLevel RespMesg) (cp: FifoHighLevel RespMesg).
+  Import Classical.
+  Import RespMesg.
 
-Section classic.
-  Hypothesis dec : forall P, P \/ ~ P.
+  Definition send pt m t :=
+    match pt with
+      | p => pc.enq m t
+      | c => cp.enq m t
+    end.
+  
+  Definition recv pt m t :=
+    match pt with
+      | p => cp.deq m t
+      | c => pc.deq m t
+    end.
 
-  Section fifo.
-    Hypothesis uniqueEnq:
-      forall s m n t1 t2, enq s m t1 -> enq s n t2 -> ((m = n -> t1 = t2) /\ (t1 = t2 -> m = n)).
+  Parameter state: Point -> nat -> State.
+  Definition nextState pt t := state pt (S t).
 
-    Hypothesis uniqueDeq:
-      forall s m n t1 t2, deq s m t1 -> deq s n t2 -> ((m = n -> t1 = t2) /\ (t1 = t2 -> m = n)).
+  Axiom init: state p 0 = state c 0.
+  Axiom stateChange: forall {pt t}, state pt t <> nextState pt t -> exists m, send pt m t \/ recv pt m t.
 
-    Hypothesis deqImpEnq:
-      forall s m t, deq s m t -> exists t', t' <= t /\ enq s m t'.
+  Axiom sendCommon: forall {pt m t}, send pt m t -> state pt t = fst m /\ nextState pt t = snd m.
 
-    Hypothesis fifo:
-      forall s m te td, deq s m td -> enq s m te -> forall m' te' td', deq s m' td' -> enq s m' te' -> ((td' < td -> te' < te) /\ (te' < te -> td' < td)).
+  Axiom recvParent: forall {m t}, recv p m t -> nextState p t = snd m.
 
-    Theorem fifo':
-      forall {s m te td}, deq s m td -> enq s m te -> forall {m' te' td'}, deq s m' td' -> enq s m' te' -> ((td' <= td -> te' <= te) /\ (te' <= te -> td' <= td)).
-      Proof.
-        intros.
-        pose proof (fifo s m te td H H0 m' te' td' H1 H2).
-        destruct H3.
-        constructor.
-        intros.
-        assert (td' < td \/ td' >= td) by crush.
-        destruct H6.
-        specialize (H3 H6).
-        crush.
-        assert (td = td') by crush.
-        pose proof (uniqueDeq s m m' td td' H H1).
-        destruct H8.
-        specialize (H9 H7).
-        pose proof (uniqueEnq s m m' te te' H0 H2).
-        destruct H10.
-        specialize (H10 H9).
-        crush.
-        intros.
-        assert (te' < te \/ te' >= te) by crush.
-        destruct H6.
-        specialize (H4 H6).
-        crush.
-        assert (te = te') by crush.
-        pose proof (uniqueEnq s m m' te te' H0 H2).
-        destruct H8.
-        specialize (H9 H7).
-        pose proof (uniqueDeq s m m' td td' H H1).
-        destruct H10.
-        specialize (H10 H9).
-        crush.
-      Qed.
+  Axiom recvChildChange: forall {m t}, recv c m t -> fst m <= state c t -> nextState c t = snd m.
 
-    Theorem send0Fifo:
-      forall {s m t}, enq s m 0 -> deq s m t -> forall t', t' < t -> forall {m'}, ~ deq s m' t'.
+  Axiom recvChildNoChange: forall {m t}, recv c m t -> fst m > state c t -> nextState c t = state c t.
+
+  Axiom sendParent: forall {m t}, send p m t -> fst m < snd m.
+
+  Axiom sendChild: forall {m t}, send c m t -> fst m > snd m.
+
+  Section noRecvParent.
+    Context {ti : nat}.
+
+    Lemma noRecvParentNow {t} (noRecv : forall m, ~ recv p m t) : nextState p t >= state p t.
     Proof.
-      unfold not.
-      intros.
-      specialize (deqImpEnq s m' t' H2).
-      destruct deqImpEnq.
-      destruct H3.
-      specialize (fifo s m 0 t H0 H m' x t' H2 H4).
+      assert (eqOrNot: state p t = nextState p t \/ state p t <> nextState p t) by decide equality.
+      destruct eqOrNot as [eq | notEq].
+      crush.
+      pose proof (stateChange notEq) as exMsg.
+      destruct exMsg as [m sendOrRecv].
+      destruct sendOrRecv as [sendM | recvM].
+      pose proof (sendCommon sendM) as rel1.
+      pose proof (sendParent sendM) as rel2.
+      assert (state p t < nextState p t) by crush.
+      crush.
+      specialize (noRecv m recvM); crush.
+    Qed.
+
+    Lemma noRecvParent' {td} (noRecv : forall t, ti <= t <= ti + td -> forall m, ~ recv p m t):
+      nextState p (ti + td) >= state p ti.
+    Proof.
+      induction td.
+      assert (noRecvTi: forall m, ~ recv p m ti) by (unfold not; intro m; intro recvM; assert (cond: ti <= ti <= ti + 0) by crush; specialize (noRecv ti cond m); crush).
+      assert (nextState p ti >= state p ti) by (apply (noRecvParentNow noRecvTi)).
+      assert (ti + 0 = ti) by crush.
+      crush.
+      assert (indNoRecv: forall t, ti <= t <= ti + td -> forall m, ~ recv p m t) by (
+        intro t; intro cond; intro m; assert (cond': ti <= t <= ti + S td) by crush; apply (noRecv t cond' m)).
+      specialize (IHtd indNoRecv).
+      clear indNoRecv.
+      assert (noRecvNow: forall m, ~ recv p m (ti + S td)) by (
+        intros; assert (cond: ti <= ti + S td <= ti + S td) by crush; apply (noRecv (ti + S td) cond m)).
+      pose proof (noRecvParentNow noRecvNow) as stateRel.
+      assert (state p (ti + S td) = nextState p (ti + td)) by (unfold nextState; crush).
       crush.
     Qed.
 
-    Section message.
-      Parameter state : Point -> Time -> State.
+    Lemma noRecvParent1 {tf} (tiLeTf: ti <= tf) (noRecv: forall t, ti <= t <= tf -> forall m, ~ recv p m t): nextState p tf >= state p ti.
+    Proof.
+      pose proof (@noRecvParent' (tf - ti)) as noRecvParentInst.      assert (rew: ti + (tf - ti) = tf) by crush.
+      rewrite rew in noRecvParentInst.
+      firstorder.
+    Qed.
+  End noRecvParent.
 
-      Definition nextState pt t := state pt (S t).
+  Lemma noRecvParent2 {ti tf}:
+    ti <= tf -> (forall t, S ti <= t <= tf -> forall m, ~ recv p m t) ->
+    nextState p tf >= nextState p ti.
+  Proof.
+    intros.
+    assert (dec: S ti <= tf \/ ti = tf) by crush.
+    destruct dec.
+    apply noRecvParent1; crush.
+    crush.
+  Qed.
 
-      Hypothesis init: state p 0 = state c 0.
+  Lemma zeroRecvParent {m} (sendM: send c m 0) {t} (recvM: recv p m t) {t'} (le: t' <= t):
+    state p t' >= state p 0.
+  Proof.
+    pose proof (cp.enq0First sendM recvM) as enqFirst'.
+    destruct t'.
+    crush.
+    assert (enqFirst: forall t1, 0 <= t1 <= t' -> forall m', ~ recv p m' t1) by (intros; assert (t1 < t) by crush; firstorder).
+    apply noRecvParent1; crush.
+  Qed.
 
-      Hypothesis stateChange : forall pt t, state pt t <> nextState pt t -> exists m, sendm pt m t \/ recvm pt m t.
+  Section noRecvChild.
+    Context {ti : nat}.
 
-      Hypothesis sendCommon: forall pt m t, sendm pt m t -> state pt t = fst m /\ nextState pt t = snd m.
+    Lemma noRecvChildNow {t} (noRecv : forall m, ~ (recv c m t /\ fst m <= state c t)):
+      nextState c t <= state c t.
+    Proof.
+      assert (eqOrNot: state c t = nextState c t \/ state c t <> nextState c t) by decide equality.
+      destruct eqOrNot as [eq | notEq].
+      crush.
+      pose proof (stateChange notEq) as exMsg.
+      destruct exMsg as [m rest].
+      destruct rest as [sendM | recvM].
+      pose proof (sendCommon sendM) as rel1.
+      pose proof (sendChild sendM) as rel2.
+      assert (state c t > nextState c t) by crush.
+      crush.
+      specialize (noRecv m).
+      assert (decLe: fst m <= state c t \/ fst m > state c t) by crush.
+      destruct decLe as [le | gt].
+      crush.
+      assert (nextState c t = state c t) by (apply (recvChildNoChange recvM gt)).
+      crush.
+    Qed.
 
-      Hypothesis recvParent: forall m t, recvm p m t -> nextState p t = snd m.
+    Lemma noRecvChild' {td} (noRecv: forall t, ti <= t <= ti + td -> forall m, ~ (recv c m t /\ fst m <= state c t)):
+      nextState c (ti + td) <= state c ti.
+    Proof.
+      induction td.
+      assert (noRecvTi: forall m, ~ (recv c m ti /\ fst m <= state c ti)) by (unfold not; intro m; intro recvM; assert (cond: ti <= ti <= ti + 0) by crush; specialize (noRecv ti cond m recvM); crush).
+      assert (nextState c ti <= state c ti) by (apply (noRecvChildNow noRecvTi)).
+      assert (ti + 0 = ti) by crush.
+      crush.
+      assert (indNoRecv: forall t, ti <= t <= ti + td -> forall m, ~ (recv c m t /\ fst m <= state c t)) by (
+        intro t; intro cond; intro m; assert (cond': ti <= t <= ti + S td) by crush; apply (noRecv t cond' m)).
+      specialize (IHtd indNoRecv).
+      clear indNoRecv.
+      assert (noRecvNow: forall m, ~ (recv c m (ti + S td) /\ fst m <= state c (ti + S td))) by (
+        intros; assert (cond: ti <= ti + S td <= ti + S td) by crush; apply (noRecv (ti + S td) cond m)).
+      pose proof (noRecvChildNow noRecvNow) as stateRel.
+      assert (state c (ti + S td) = nextState c (ti + td)) by (unfold nextState; crush).
+      crush.
+    Qed.
 
-      Hypothesis recvChildChange  : forall m t, recvm c m t -> fst m <= state c t -> nextState c t = snd m.
+    Lemma noRecvChild1 {tf} (tiLeTf: ti <= tf) (noRecv: forall t, ti <= t <= tf -> forall m, ~ (recv c m t /\ fst m <= state c t)): nextState c tf <= state c ti.
+    Proof.
+      pose proof (@noRecvChild' (tf - ti)) as noRecvChildInst.
+      assert (rew: ti + (tf - ti) = tf) by crush.
+      rewrite rew in noRecvChildInst.
+      firstorder.
+    Qed.
+  End noRecvChild.
 
-      Hypothesis recvChildNoChange: forall m t, recvm c m t -> fst m > state c t -> nextState c t = state c t.
+  Lemma noRecvChild2 {ti tf}:
+    ti <= tf -> (forall t, S ti <= t <= tf -> forall m, ~ (recv c m t /\ fst m <= state c t)) ->
+    nextState c tf <= nextState c ti.
+  Proof.
+    intros.
+    assert (dec: S ti <= tf \/ ti = tf) by crush.
+    destruct dec.
+    apply noRecvChild1; crush.
+    crush.
+  Qed.
 
-      Hypothesis sendParent: forall m t, sendm p m t -> fst m < snd m.
+  Lemma childRecv {ti tf} (le: ti <= tf) (nscTiLtTf: nextState c ti < nextState c tf):
+    exists t, S ti <= t <= tf /\ exists m, recv c m t /\ fst m <= state c t.
+  Proof.
+    pose proof (noRecvChild2 le) as noRecv.
+    assert (gt: ~ nextState c tf <= nextState c ti) by crush.
+    pose proof (dec (exists t, S ti <= t <= tf /\ exists m, recv c m t /\ fst m <= state c t)) as exDec.
+    firstorder.
+  Qed.
 
-      Hypothesis sendChild: forall m t, sendm c m t -> fst m > snd m.
+  Lemma zeroRecvChild {m} (sendM: send p m 0) {t} (recvM: recv c m t) {t'} (le: t' <= t):
+    state c t' <= state c 0.
+  Proof.
+    
+    pose proof (pc.enq0First sendM recvM) as enqFirst'.
+    destruct t'.
+    crush.
+    assert (enqFirst: forall t1, 0 <= t1 <= t' -> forall m', ~ (recv c m' t1 /\ fst m' <= state c t1)) by (intros; assert (t1 < t) by crush; firstorder).
+    apply noRecvChild1; crush.
+  Qed.
 
-      Section noRecvParent.
-        Context {ti : nat}.
+  Lemma childRecvNoParentRecv {tp tc} (recvpImpSendc: forall m t1 t2, recv p m t1 -> send c m t2 -> t1 <= tp -> t2 <= tc) (recvcImpSendp: forall m t1 t2, recv c m t1 -> send p m t2 -> t1 <= tc -> t2 <= tp) {tr} (trLeTc: tr <= tc) {m} (recvcm: recv c m tr /\ fst m <= state c tr) (noRecvc: forall t, S tr <= t <= tc -> ~ exists m, recv c m t /\ fst m <= state c t) {ts} (sendp: send p m ts) (noRecvp: forall t, S ts <= t <= tp -> forall m, ~ recv p m t) (contra: nextState c tc > nextState p tp): False.
+    assert (noRecvc': forall t, S tr <= t <= tc -> forall m, ~ (recv c m t /\ fst m <= state c t)) by (generalize noRecvc; clear; firstorder).
+    clear noRecvc.
+    assert (nscTcLeTr: nextState c tc <= nextState c tr) by (apply (noRecvChild2 trLeTc noRecvc')).
+    assert (tsLeTp: ts <= tp) by (apply (recvcImpSendp m tr); crush).
+    assert (nspTpGeTs: nextState p tp >= nextState p ts) by (apply (noRecvParent2 tsLeTp noRecvp)).
+    assert (nextState p ts = snd m) by (apply sendCommon; crush).
+    assert (nextState c tr = snd m) by (apply recvChildChange; crush).
+    crush.
+  Qed.
 
-        Lemma noRecvParentNow {t} (noRecv : forall m, ~ recvm p m t) : nextState p t >= state p t.
-        Proof.
-          destruct (dec (state p t = nextState p t)).
-          crush.
-          pose proof (stateChange p t H).
-          destruct H0.
-          destruct H0.
-          pose proof (sendCommon p x t H0).
-          pose proof (sendParent x t H0).
-          assert (state p t < nextState p t) by crush.
-          crush.
-          specialize (noRecv x H0).
-          crush.
-        Qed.
+  Theorem strongLess:
+    forall tp tc,
+      (forall m t1 t2, recv p m t1 -> send c m t2 -> t1 <= tp -> t2 <= tc) ->
+      (forall m t1 t2, recv c m t1 -> send p m t2 -> t1 <= tc -> t2 <= tp) ->
+      ~ (nextState c tc > nextState p tp).
+  Proof.
+    apply (notExistForallNot dec).
+    unfold not.
+    intros exStmt.
+    pose proof (minExists2 dec exStmt) as exMin.
+    clear exStmt.
+    destruct exMin as [tpmin exMin].
+    destruct exMin as [tcmin exMin].
+    destruct exMin as [ex min].
+    destruct min as [tpminHyp' tcminHyp'].
+    destruct ex as [pRecvCSend rest].
+    destruct rest as [cRecvPSend wrongState].
+    assert (tpminHyp: ~ exists x y, x < tpmin /\
+      (forall m t1 t2, recv p m t1 -> send c m t2 -> t1 <= x -> t2 <= y) /\
+      (forall m t1 t2, recv c m t1 -> send p m t2 -> t1 <= y -> t2 <= x) /\
+      nextState c y > nextState p x) by firstorder.
+    clear tpminHyp'.
+    clear tcminHyp'.
+    destruct (dec (forall t, 0 <= t <= tpmin -> forall m, ~ recv p m t)) as [pNotRecv | pRecv'].
+    destruct (dec (forall t, 0 <= t <= tcmin -> forall m, ~ (recv c m t /\ fst m <= state c t))) as [cNotRecv | cRecv'].
+    assert (zeroLeTpmin: 0 <= tpmin) by crush.
+    assert (nsPTpminGeStateP0: nextState p tpmin >= state p 0) by (apply (noRecvParent1 zeroLeTpmin pNotRecv)).
+    clear pNotRecv zeroLeTpmin.
+    assert (zeroLeTcmin: 0 <= tcmin) by crush.
+    assert (nsCTcminLeStateC0: nextState c tcmin <= state c 0) by (apply (noRecvChild1 zeroLeTcmin cNotRecv)).
+    assert (nsCTcminLeNsPTpmin: nextState c tcmin <= nextState p tpmin) by (pose proof init; crush).
+    crush.
+    assert (cRecvEx: exists t, 0 <= t <= tcmin /\ exists m, recv c m t /\ fst m <= state c t) by (generalize (dec (exists t, 0 <= t <= tcmin /\ exists m, recv c m t /\ fst m <= state c t)) cRecv'; clear; firstorder).
+    clear cRecv'.
+    destruct cRecvEx as [tcRecv rest].
+    assert (cRecv: exists x, x <= tcmin /\ exists m, recv c m x /\ fst m <= state c x) by (exists tcRecv; crush).
+    clear tcRecv rest.
+    pose proof (maxExists dec cRecv) as cRecvMax.
+    clear cRecv.
+    destruct cRecvMax as [tcmax rest].
+    destruct rest as [tcmaxLeTcmin rest].
+    destruct rest as [cRecvMax noCRecv].
+    destruct cRecvMax as [m childRecvCond].
+    assert (exTpmax: exists tpmax, tpmax <= tcmax /\ send p m tpmax) by (apply pc.deqImpEnq; crush).
+    destruct exTpmax as [tpmax rest].
+    destruct rest as [useless sendPMTpmax].
+    clear useless.
+    assert (pNotRecvGtTpmax: forall t, S tpmax <= t <= tpmin -> forall m, ~ recv p m t) by
+      (intros; assert (0 <= t <= tpmin) by crush; apply pNotRecv; crush).
+    apply (childRecvNoParentRecv pRecvCSend cRecvPSend tcmaxLeTcmin childRecvCond noCRecv sendPMTpmax pNotRecvGtTpmax wrongState).
+    assert (pRecv'': exists t, 0 <= t <= tpmin /\ exists m, recv p m t) by (generalize (dec (exists t, 0 <= t <= tpmin /\ exists m, recv p m t)) pRecv'; clear; firstorder).
+    clear pRecv'.
+    assert (exPRecv: exists t, t <= tpmin /\ exists m, recv p m t) by (destruct pRecv'' as [t rest]; exists t; crush).
+    clear pRecv''.
+    pose proof (maxExists dec exPRecv) as exPRecvMax.
+    clear exPRecv.
+    destruct exPRecvMax as [tp1 rest].
+    destruct rest as [tp1LeTpmin rest].
+    destruct rest as [exM noRecvGTTp1'].
+    destruct exM as [m recvmPMTp1].
+    assert (noRecvGTTp1: forall y, S tp1 <= y <= tpmin -> forall m, ~ recv p m y) by (generalize noRecvGTTp1'; clear; firstorder).
+    clear noRecvGTTp1'.
+    assert (nsPTpminGeNsPTp1: nextState p tpmin >= nextState p tp1) by (apply noRecvParent2; crush).
+    assert (exRest: exists tc1, tc1 <= tp1 /\ send c m tc1) by (apply cp.deqImpEnq; crush).
+    destruct exRest as [tc1 rest].
+    destruct rest as [tc1LeTp1 sendmCMTc1].
 
-        Lemma noRecvParent' {td} (noRecv : forall t, ti <= t <= ti + td -> forall m, ~ recvm p m t):
-          nextState p (ti + td) >= state p ti.
-        Proof.
-          induction td.
-          assert (forall m, ~ recvm p m ti).
-          unfold not.
-          intros.
-          assert (ti <= ti <= ti + 0) by crush.
-          specialize (noRecv ti H0 m).
-          crush.
-          assert (nextState p ti >= state p ti) by (apply (noRecvParentNow H)).
-          assert (ti + 0 = ti) by crush.
-          crush.
-          assert (forall t, ti <= t <= ti + td -> forall m, ~ recvm p m t).
-          intros.
-          assert (ti <= t <= ti + S td) by crush.
-          apply (noRecv t H0 m).
-          specialize (IHtd H).
-          clear H.
-          assert (forall m, ~ recvm p m (ti + S td)).
-          intros.
-          assert (ti <= ti + S td <= ti + S td) by crush.
-          apply (noRecv (ti + S td) H m).
-          pose proof (noRecvParentNow H).
-          assert (ti + S td = S (ti + td)) by crush.
-          unfold nextState in IHtd.
-          assert (state p (S (ti + td)) = state p (ti + S td)) by crush.
-          assert (state p (ti + S td) >= state p ti) by crush.
-          crush.
-        Qed.
+    assert (rest: state c tc1 = fst m /\ nextState c tc1 = snd m) by (apply sendCommon; crush).
+    destruct rest as [sCTc1EqFstM nsCTc1EqSndM].
+    assert (nsCTcminGTNsPTp1: nextState c tcmin > nextState p tp1) by crush.
+    assert (nsPTp1EqSndM: nextState p tp1 = snd m) by (apply recvParent; crush).
+    assert (nsCTc1LtNsCTcmin: nextState c tc1 < nextState c tcmin) by crush.
+    assert (tc1LeTcmin: tc1 <= tcmin) by (apply (pRecvCSend m tp1); crush).
+    pose proof (childRecv tc1LeTcmin nsCTc1LtNsCTcmin) as exCRecv.
 
-        Lemma noRecvParent1 {tf}:
-          ti <= tf -> (forall t, ti <= t <= tf -> forall m, ~ recvm p m t) ->
-          nextState p tf >= state p ti.
-        Proof.
-          intros.
-          pose proof (@noRecvParent' (tf - ti)).
-          assert (ti + (tf - ti) = tf) by crush.
-          assert (forall t, ti <= t <= ti + (tf - ti) -> forall m, ~ recvm p m t).
-          intros.
-          assert (ti <= t <= tf) by crush.
-          specialize (H0 t H4 m).
-          crush.
-          crush.
-        Qed.
-      End noRecvParent.
+    assert (sCTc1GtNsCTc1: state c tc1 > nextState c tc1) by (assert (fst m > snd m) by (apply (@sendChild m tc1); crush); crush).
 
-      Lemma noRecvParent2 {ti tf}:
-        ti <= tf -> (forall t, S ti <= t <= tf -> forall m, ~ recvm p m t) ->
-        nextState p tf >= nextState p ti.
-      Proof.
-        intros.
-        assert (S ti <= tf \/ ti = tf) by crush.
-        destruct H1.
-        apply noRecvParent1; crush.
-        crush.
-      Qed.
+    clear nsPTpminGeNsPTp1 sCTc1EqFstM nsCTc1EqSndM nsCTcminGTNsPTp1 nsPTp1EqSndM nsCTc1LtNsCTcmin.
 
-      Lemma zeroRecvParent:
-        forall {m t}, sendm c m 0 -> recvm p m t -> forall t', t' <= t -> state p t' >= state p 0.
-      Proof.
-        intros.
-        pose proof (send0Fifo H H0).
-        destruct t'.
-        crush.
-        assert (forall t1, 0 <= t1 <= t' -> forall m', ~ recvm p m' t1) by (intros; assert (t1 < S t) by crush; apply H2; crush).
-        apply noRecvParent1; crush.
-      Qed.
+    pose proof (minExists dec exCRecv) as exCRecvMin.
 
-      Section noRecvChild.
-        Context {ti : nat}.
+    clear exCRecv.
+    destruct exCRecvMin as [tc2 rest].
+    destruct rest as [rest noCRecvGTTc1'].
+    destruct rest as [tc1LtTc2LeTcmin exCRecv].
+    generalize exCRecv; intro rest.
+    destruct rest as [n rest].
+    destruct rest as [cRecvN fstN].
+    assert (exPSend: exists tp2, tp2 <= tc2 /\ send p n tp2) by (apply pc.deqImpEnq; crush).
+    destruct exPSend as [tp2 rest].
+    destruct rest as [tp2LeTc2 pSendN].
+    assert (fstSndPN: state p tp2 = fst n /\ nextState p tp2 = snd n) by (apply sendCommon; crush).
+    destruct fstSndPN as [fstPN sndPN].
+    assert (sPTp2LeScTc2: state p tp2 <= state c tc2) by crush.
 
-        Lemma noRecvChildNow {t} (noRecv : forall m, ~ (recvm c m t /\ fst m <= state c t)):
-          nextState c t <= state c t.
-        Proof.
-          destruct (dec (state c t = nextState c t)).
-          crush.
-          pose proof (stateChange c t H).
-          destruct H0.
-          destruct H0.
-          pose proof (sendCommon c x t H0).
-          pose proof (sendChild x t H0).
-          assert (state c t > nextState c t) by crush.
-          crush.
-          specialize (noRecv x).
-          destruct (dec (fst x <= state c t)).
-          crush.
-          assert (fst x > state c t) by crush.
-          assert (nextState c t = state c t) by (apply (recvChildNoChange x t H0 H2)).
-          crush.
-        Qed.
+    destruct tc2.
+    crush.
+    assert (tc1LeTc2: tc1 <= tc2) by crush.
+    assert (noCRecv': forall y, S tc1 <= y <= tc2 -> ~ exists m, recv c m y /\ fst m <= state c y) by
+      (intro; intro hyp; assert (hyp': y < S tc2) by (generalize hyp; clear; crush); specialize (noCRecvGTTc1' y hyp'); assert (S tc1 <= y <= tcmin) by (generalize hyp tc1LtTc2LeTcmin; clear; crush); crush).
+    assert (noCRecv: forall y, S tc1 <= y <= tc2 -> forall m, ~ (recv c m y /\ fst m <= state c y)) by
+      (generalize noCRecv'; clear; firstorder).
+    clear noCRecv'.
+    pose proof (noRecvChild2 tc1LeTc2 noCRecv) as nsCtc2LeNsCTc1.
+    assert (sCTc1GtSPTp2: state c tc1 > state p tp2) by (generalize sCTc1GtNsCTc1 sPTp2LeScTc2 nsCtc2LeNsCTc1; clear; unfold nextState in *; crush).
+    clear noCRecvGTTc1'.
+    clear sCTc1GtNsCTc1 fstPN sndPN sPTp2LeScTc2 nsCtc2LeNsCTc1.
 
-        Lemma noRecvChild' {td} (noRecv : forall t, ti <= t <= ti + td -> forall m, ~ (recvm c m t /\ fst m <= state c t)) :
-          nextState c (ti + td) <= state c ti.
-        Proof.
-          induction td.
-          assert (forall m, ~ (recvm c m ti /\ fst m <= state c ti)).
-          unfold not.
-          intros.
-          assert (ti <= ti <= ti + 0) by crush.
-          specialize (noRecv ti H0 m).
-          crush.
-          assert (nextState c ti <= state c ti) by (apply (noRecvChildNow H)).
-          assert (ti + 0 = ti) by crush.
-          crush.
-          assert (forall t, ti <= t <= ti + td -> forall m, ~ (recvm c m t /\ fst m <= state c t)).
-          intros.
-          assert (ti <= t <= ti + S td) by crush.
-          apply (noRecv t H0 m).
-          specialize (IHtd H).
-          clear H.
-          assert (forall m, ~ (recvm c m (ti + S td) /\ fst m <= state c (ti + S td))).
-          intros.
-          assert (ti <= ti + S td <= ti + S td) by crush.
-          apply (noRecv (ti + S td) H m).
-          pose proof (noRecvChildNow H).
-          assert (ti + S td = S (ti + td)) by crush.
-          unfold nextState in IHtd.
-          assert (state c (S (ti + td)) = state c (ti + S td)) by crush.
-          assert (state c (ti + S td) <= state c ti) by crush.
-          crush.
-        Qed.
+    assert (tp1LeTp2OrNot: tp1 <= tp2 \/ tp2 < tp1) by (clear; crush).
+    destruct tp1LeTp2OrNot as [tp1LeTp2 | tp2LtTp1].
+    assert (tc2LtTcmin: S tc2 <= tcmin) by crush.
+    pose proof (@maxExistsPower dec (fun t => exists m, recv c m t /\ fst m <= state c t) tcmin (S tc2) tc2LtTcmin exCRecv) as exCRecvMax.
+    destruct exCRecvMax as [tc3 rest].
+    destruct rest as [tc2LtTc3LeTcmin rest].
+    destruct rest as [exCRecvTc3 noCRecvGtTc3].
+    destruct exCRecvTc3 as [n' cRecvTc3Fst].
+    generalize cRecvTc3Fst; intro hyp.
+    destruct hyp as [cRecvTc3 fstTc3].
+    assert (tc2LtTc3: S tc2 <= tc3) by crush.
+    assert (exPRecvTp3: exists tp3, tp3 <= tc3 /\ send p n' tp3) by (apply pc.deqImpEnq; crush).
+    destruct exPRecvTp3 as [tp3 rest].
+    destruct rest as [junk pSendX].
+    clear junk.
+    pose proof (pc.fifo2' pSendX cRecvTc3 pSendN cRecvN) as impTp2LeTp3.
+    specialize (impTp2LeTp3 tc2LtTc3).
+    assert (noRecvPLate: forall y, S tp3 <= y <= tpmin -> forall m, ~ recv p m y) by
+      (intros; assert (hyp: S tp1 <= y <= tpmin) by crush; generalize y hyp noRecvGTTp1; clear; firstorder).
+    assert (tc3LeTcmin: tc3 <= tcmin) by crush.
+    pose proof (childRecvNoParentRecv pRecvCSend cRecvPSend tc3LeTcmin cRecvTc3Fst noCRecvGtTc3 pSendX noRecvPLate).
+    crush.
 
-        Lemma noRecvChild1 {tf}:
-          ti <= tf -> (forall t, ti <= t <= tf -> forall m, ~ (recvm c m t /\ fst m <= state c t)) ->
-          nextState c tf <= state c ti.
-        Proof.
-          intros.
-          pose proof (@noRecvChild' (tf - ti)).
-          assert (ti + (tf - ti) = tf) by crush.
-          assert (forall t, ti <= t <= ti + (tf - ti) -> forall m, ~ (recvm c m t /\ fst m <= state c t)).
-          intros.
-          assert (ti <= t <= tf) by crush.
-          specialize (H0 t H4 m).
-          crush.
-          crush.
-        Qed.
-      End noRecvChild.
+    destruct tp2.
+    assert (tc1LeSTc2: tc1 <= S tc2) by crush.
+    pose proof (zeroRecvChild pSendN cRecvN tc1LeSTc2) as contra1.
+    clear tc1LeSTc2.
+    pose proof init.
+    crush.
 
-      Lemma noRecvChild2 {ti tf}:
-        ti <= tf -> (forall t, S ti <= t <= tf -> forall m, ~ (recvm c m t /\ fst m <= state c t)) ->
-        nextState c tf <= nextState c ti.
-      Proof.
-        intros.
-        assert (S ti <= tf \/ ti = tf) by crush.
-        destruct H1.
-        apply noRecvChild1; crush.
-        crush.
-      Qed.
+    destruct tc1.
+    assert (sTp2LeTp1: S tp2 <= tp1) by crush.
+    pose proof (zeroRecvParent sendmCMTc1 recvmPMTp1 sTp2LeTp1) as contra2.
+    clear sTp2LeTp1.
+    pose proof init.
+    crush.
 
-      Lemma childRecv {ti tf}:
-        ti <= tf -> nextState c ti < nextState c tf -> exists t, S ti <= t <= tf /\ exists m, recvm c m t /\ fst m <= state c t.
-      Proof.
-        intros.
-        pose proof (noRecvChild2 H).
-        assert (~ nextState c tf <= nextState c ti) by crush.
-        generalize H2 H1 (dec (exists t, S ti <= t <= tf /\ exists m, recvm c m t /\ fst m <= state c t)).
-        clear.
-        intros.
-        firstorder.
-      Qed.
+    destruct tp1.
+    crush.
 
-      Lemma zeroRecvChild:
-        forall {m t}, sendm p m 0 -> recvm c m t -> forall t', t' <= t -> state c t' <= state c 0.
-      Proof.
-        intros.
-        pose proof (send0Fifo H H0).
-        destruct t'.
-        crush.
-        assert (forall t1, 0 <= t1 <= t' -> forall m', ~ (recvm c m' t1 /\ fst m' <= state c t1)) by (intros; assert (t1 < S t) by crush; unfold not; intro dep; destruct dep as [one two]; generalize one; apply H2; crush).
-        apply noRecvChild1; crush.
-      Qed.
+    assert (hyp1: forall k t1 t2, recv p k t1 -> send c k t2 -> t1 <= tp2 -> t2 <= tc1).
+    intros.
+    pose proof @cp.fifo1.
+    assert (useful: t1 < S tp1 -> t2 < S tc1) by (apply (@cp.fifo2 m (S tc1) (S tp1) sendmCMTc1 recvmPMTp1 k); crush).
+    assert (lt1: tc1 < S tp1) by crush.
+    assert (lt2: t1 < S tp1) by crush.
+    clear lt1.
+    specialize (useful lt2).
+    crush.
 
-      Lemma childRecvNoParentRecv {tp tc}:
-        (forall m t1 t2, recvm p m t1 -> sendm c m t2 -> t1 <= tp -> t2 <= tc) ->
-        (forall m t1 t2, recvm c m t1 -> sendm p m t2 -> t1 <= tc -> t2 <= tp) ->
-        forall {tr}, tr <= tc -> forall {m}, (recvm c m tr /\ fst m <= state c tr) ->
-          (forall t, S tr <= t <= tc -> ~ exists m', recvm c m' t /\ fst m' <= state c t) ->
-          forall {ts}, sendm p m ts -> (forall t', S ts <= t' <= tp -> forall m'', ~ recvm p m'' t') ->
-        ~ (nextState c tc > nextState p tp).
-        unfold not.
-        intros.
-        assert (forall t, S tr <= t <= tc -> forall m', ~ (recvm c m' t /\ fst m' <= state c t)) by (generalize H3; clear; firstorder).
-        clear H3.
-        assert (nextState c tc <= nextState c tr) by (apply (noRecvChild2 H1 H7)).
-        assert (ts <= tp) by (apply (H0 m tr); crush).
-        assert (nextState p tp >= nextState p ts) by (apply (noRecvParent2 H8 H5)).
-        assert (nextState p ts = snd m) by (apply sendCommon; crush).
-        assert (nextState c tr = snd m) by (apply recvChildChange; crush).
-        crush.
-      Qed.
+    assert (hyp2: forall k t1 t2, recv c k t1 -> send p k t2 -> t1 <= tc1 -> t2 <= tp2).
+    intros.
+    assert (useful: t1 < S tc2 -> t2 < S tp2) by (apply (@pc.fifo2 n (S tp2) (S tc2)pSendN cRecvN k); crush).
+    assert (lt1: tc1 < S tc2) by crush.
+    assert (lt2: t1 < S tc2) by crush.
+    clear lt1.
+    specialize (useful lt2).
+    crush.
 
-      Theorem strongLess:
-        forall tp tc,
-          (forall m t1 t2, recvm p m t1 -> sendm c m t2 -> t1 <= tp -> t2 <= tc) ->
-          (forall m t1 t2, recvm c m t1 -> sendm p m t2 -> t1 <= tc -> t2 <= tp) ->
-          ~ (nextState c tc > nextState p tp).
-      Proof.
-        apply (notExistForallNot dec).
-        unfold not.
-        intros exStmt.
-        pose proof (minExists2 dec exStmt) as exMin.
-        clear exStmt.
-        destruct exMin as [tpmin exMin].
-        destruct exMin as [tcmin exMin].
-        destruct exMin as [ex min].
-        destruct min as [tpminHyp' tcminHyp'].
-        destruct ex as [pRecvCSend rest].
-        destruct rest as [cRecvPSend wrongState].
-        assert (tpminHyp: ~ exists x y, x < tpmin /\
-          (forall m t1 t2, recvm p m t1 -> sendm c m t2 -> t1 <= x -> t2 <= y) /\
-          (forall m t1 t2, recvm c m t1 -> sendm p m t2 -> t1 <= y -> t2 <= x) /\
-          nextState c y > nextState p x) by firstorder.
-        clear tpminHyp'.
-        assert (tcminHyp: ~ exists y, y < tcmin /\
-          (forall m t1 t2, recvm p m t1 -> sendm c m t2 -> t1 <= tpmin -> t2 <= y    ) /\
-          (forall m t1 t2, recvm c m t1 -> sendm p m t2 -> t1 <= y     -> t2 <= tpmin) /\
-          nextState c y > nextState p tpmin) by firstorder.
-        clear tcminHyp'.
-        destruct (dec (forall t, 0 <= t <= tpmin -> forall m, ~ recvm p m t)) as [pNotRecv | pRecv'].
-        destruct (dec (forall t, 0 <= t <= tcmin -> forall m, ~ (recvm c m t /\ fst m <= state c t))) as [cNotRecv | cRecv'].
-        assert (zeroLeTpmin: 0 <= tpmin) by crush.
-        assert (nsPTpminGeStateP0: nextState p tpmin >= state p 0) by (apply (noRecvParent1 zeroLeTpmin pNotRecv)).
-        clear pNotRecv zeroLeTpmin.
-        assert (zeroLeTcmin: 0 <= tcmin) by crush.
-        assert (nsCTcminLeStateC0: nextState c tcmin <= state c 0) by (apply (noRecvChild1 zeroLeTcmin cNotRecv)).
-        assert (nsCTcminLeNsPTpmin: nextState c tcmin <= nextState p tpmin) by crush.
-        crush.
-        assert (cRecvEx: exists t, 0 <= t <= tcmin /\ exists m, recvm c m t /\ fst m <= state c t) by (generalize (dec (exists t, 0 <= t <= tcmin /\ exists m, recvm c m t /\ fst m <= state c t)) cRecv'; clear; firstorder).
-        clear cRecv'.
-        destruct cRecvEx as [tcRecv rest].
-        assert (cRecv: exists x, x <= tcmin /\ exists m, recvm c m x /\ fst m <= state c x) by (exists tcRecv; crush).
-        clear tcRecv rest.
-        pose proof (maxExists dec cRecv) as cRecvMax.
-        clear cRecv.
-        destruct cRecvMax as [tcmax rest].
-        destruct rest as [tcmaxLeTcmin rest].
-        destruct rest as [cRecvMax noCRecv].
-        destruct cRecvMax as [m childRecvCond].
-        assert (exTpmax: exists tpmax, tpmax <= tcmax /\ sendm p m tpmax) by (apply deqImpEnq; crush).
-        destruct exTpmax as [tpmax rest].
-        destruct rest as [useless sendPMTpmax].
-        clear useless.
-        assert (pNotRecvGtTpmax: forall t, S tpmax <= t <= tpmin -> forall m, ~ recvm p m t) by
-          (intros; assert (0 <= t <= tpmin) by crush; apply pNotRecv; crush).
-        apply (childRecvNoParentRecv pRecvCSend cRecvPSend tcmaxLeTcmin childRecvCond noCRecv sendPMTpmax pNotRecvGtTpmax wrongState).
-        assert (pRecv'': exists t, 0 <= t <= tpmin /\ exists m, recvm p m t) by (generalize (dec (exists t, 0 <= t <= tpmin /\ exists m, recvm p m t)) pRecv'; clear; firstorder).
-        clear pRecv'.
-        assert (exPRecv: exists t, t <= tpmin /\ exists m, recvm p m t) by (destruct pRecv'' as [t rest]; exists t; crush).
-        clear pRecv''.
-        pose proof (maxExists dec exPRecv) as exPRecvMax.
-        clear exPRecv.
-        destruct exPRecvMax as [tp1 rest].
-        destruct rest as [tp1LeTpmin rest].
-        destruct rest as [exM noRecvGTTp1'].
-        destruct exM as [m recvmPMTp1].
-        assert (noRecvGTTp1: forall y, S tp1 <= y <= tpmin -> forall m, ~ recvm p m y) by (generalize noRecvGTTp1'; clear; firstorder).
-        clear noRecvGTTp1'.
-        assert (nsPTpminGeNsPTp1: nextState p tpmin >= nextState p tp1) by (apply noRecvParent2; crush).
-        assert (exRest: exists tc1, tc1 <= tp1 /\ sendm c m tc1) by (apply deqImpEnq; crush).
-        destruct exRest as [tc1 rest].
-        destruct rest as [tc1LeTp1 sendmCMTc1].
+    assert (basic: tp2 < tpmin) by crush.
 
-        assert (rest: state c tc1 = fst m /\ nextState c tc1 = snd m) by (apply sendCommon; crush).
-        destruct rest as [sCTc1EqFstM nsCTc1EqSndM].
-        assert (nsCTcminGTNsPTp1: nextState c tcmin > nextState p tp1) by crush.
-        assert (nsPTp1EqSndM: nextState p tp1 = snd m) by (apply recvParent; crush).
-        assert (nsCTc1LtNsCTcmin: nextState c tc1 < nextState c tcmin) by crush.
-        assert (tc1LeTcmin: tc1 <= tcmin) by (apply (pRecvCSend m tp1); crush).
-        pose proof (childRecv tc1LeTcmin nsCTc1LtNsCTcmin) as exCRecv.
+    clear tp1LeTpmin m recvmPMTp1 noRecvGTTp1 tc1LeTp1 sendmCMTc1 tc1LeTcmin tc1LtTc2LeTcmin exCRecv n cRecvN fstN tp2LeTc2 pSendN tc1LeTc2 noCRecv tp2LtTp1.
 
-        assert (sCTc1GtNsCTc1: state c tc1 > nextState c tc1) by (assert (fst m > snd m) by (apply (sendChild m tc1); crush); crush).
+    clear tp1 tc2.
 
-        clear nsPTpminGeNsPTp1 sCTc1EqFstM nsCTc1EqSndM nsCTcminGTNsPTp1 nsPTp1EqSndM nsCTc1LtNsCTcmin.
+    assert (exists x y, x < tpmin /\ (forall m t1 t2, recv p m t1 -> send c m t2 -> t1 <= x -> t2 <= y) /\ (forall m t1 t2, recv c m t1 -> send p m t2 -> t1 <= y -> t2 <= x) /\ nextState c y > nextState p x) by (exists tp2; exists tc1; crush).
 
-        pose proof (minExists dec exCRecv) as exCRecvMin.
+    crush.
+  Qed.
 
-        clear exCRecv.
-        destruct exCRecvMin as [tc2 rest].
-        destruct rest as [rest noCRecvGTTc1'].
-        destruct rest as [tc1LtTc2LeTcmin exCRecv].
-        generalize exCRecv; intro rest.
-        destruct rest as [n rest].
-        destruct rest as [cRecvN fstN].
-        assert (exPSend: exists tp2, tp2 <= tc2 /\ sendm p n tp2) by (apply deqImpEnq; crush).
-        destruct exPSend as [tp2 rest].
-        destruct rest as [tp2LeTc2 pSendN].
-        assert (fstSndPN: state p tp2 = fst n /\ nextState p tp2 = snd n) by (apply sendCommon; crush).
-        destruct fstSndPN as [fstPN sndPN].
-        assert (sPTp2LeScTc2: state p tp2 <= state c tc2) by crush.
+  Theorem conservative'' t:
+    ~ (nextState c t > nextState p t).
+  Proof.
+    apply strongLess.
+    intro.
+    intro.
+    intro.
+    intro recv.
+    intro send.
+    intro le.
+    pose proof (cp.deqImpEnq recv) as exEnq.
+    destruct exEnq as [t' rest].
+    destruct rest as [le2 enq].
+    pose proof (cp.uniqueEnq1 send enq) as useful.
+    crush.
+    intro.
+    intro.
+    intro.
+    intro recv.
+    intro send.
+    intro le.
+    pose proof (pc.deqImpEnq recv) as exEnq.
+    destruct exEnq as [t' rest].
+    destruct rest as [le2 enq].
+    pose proof (pc.uniqueEnq1 send enq).
+    crush.
+  Qed.
 
-        destruct tc2.
-        crush.
-        assert (tc1LeTc2: tc1 <= tc2) by crush.
-        assert (noCRecv': forall y, S tc1 <= y <= tc2 -> ~ exists m, recvm c m y /\ fst m <= state c y) by
-          (intro; intro hyp; assert (hyp': y < S tc2) by (generalize hyp; clear; crush); specialize (noCRecvGTTc1' y hyp'); assert (S tc1 <= y <= tcmin) by (generalize hyp tc1LtTc2LeTcmin; clear; crush); crush).
-        assert (noCRecv: forall y, S tc1 <= y <= tc2 -> forall m, ~ (recvm c m y /\ fst m <= state c y)) by
-          (generalize noCRecv'; clear; firstorder).
-        clear noCRecv'.
-        pose proof (noRecvChild2 tc1LeTc2 noCRecv) as nsCtc2LeNsCTc1.
-        assert (sCTc1GtSPTp2: state c tc1 > state p tp2) by (generalize sCTc1GtNsCTc1 sPTp2LeScTc2 nsCtc2LeNsCTc1; clear; unfold nextState in *; crush).
-        clear noCRecvGTTc1'.
-        clear sCTc1GtNsCTc1 fstPN sndPN sPTp2LeScTc2 nsCtc2LeNsCTc1.
+  Theorem conservative' t:
+    ~ state c t > state p t.
+  Proof.
+    destruct t.
+    unfold not; pose proof init; crush.
+    apply (@conservative'' t).
+  Qed.
 
-        assert (tp1LeTp2OrNot: tp1 <= tp2 \/ tp2 < tp1) by (clear; crush).
-        destruct tp1LeTp2OrNot as [tp1LeTp2 | tp2LtTp1].
-        assert (tc2LtTcmin: S tc2 <= tcmin) by crush.
-        pose proof (@maxExistsPower dec (fun t => exists m, recvm c m t /\ fst m <= state c t) tcmin (S tc2) tc2LtTcmin exCRecv) as exCRecvMax.
-        destruct exCRecvMax as [tc3 rest].
-        destruct rest as [tc2LtTc3LeTcmin rest].
-        destruct rest as [exCRecvTc3 noCRecvGtTc3].
-        destruct exCRecvTc3 as [n' cRecvTc3Fst].
-        generalize cRecvTc3Fst; intro hyp.
-        destruct hyp as [cRecvTc3 fstTc3].
-        assert (tc2LtTc3: S tc2 <= tc3) by crush.
-        assert (exPRecvTp3: exists tp3, tp3 <= tc3 /\ sendm p n' tp3) by (apply deqImpEnq; crush).
-        destruct exPRecvTp3 as [tp3 rest].
-        destruct rest as [junk pSendX].
-        clear junk.
-        pose proof (fifo' cRecvTc3 pSendX cRecvN pSendN) as conj.
-        destruct conj as [impTp2LeTp3 junk].
-        clear junk.
-        specialize (impTp2LeTp3 tc2LtTc3).
-        assert (noRecvPLate: forall y, S tp3 <= y <= tpmin -> forall m, ~ recvm p m y) by
-          (intros; assert (hyp: S tp1 <= y <= tpmin) by crush; generalize y hyp noRecvGTTp1; clear; firstorder).
-        assert (tc3LeTcmin: tc3 <= tcmin) by crush.
-        pose proof (childRecvNoParentRecv pRecvCSend cRecvPSend tc3LeTcmin cRecvTc3Fst noCRecvGtTc3 pSendX noRecvPLate).
-        crush.
-
-        destruct tp2.
-        assert (tc1LeSTc2: tc1 <= S tc2) by crush.
-        pose proof (zeroRecvChild pSendN cRecvN tc1 tc1LeSTc2) as contra1.
-        clear tc1LeSTc2.
-        crush.
-
-        destruct tc1.
-        assert (sTp2LeTp1: S tp2 <= tp1) by crush.
-        pose proof (zeroRecvParent sendmCMTc1 recvmPMTp1 (S tp2) sTp2LeTp1) as contra2.
-        clear sTp2LeTp1.
-        crush.
-
-        destruct tp1.
-        crush.
-
-        assert (hyp1: forall k t1 t2, recvm p k t1 -> sendm c k t2 -> t1 <= tp2 -> t2 <= tc1).
-        intros.
-        assert (big: (t1 < S tp1 -> t2 < S tc1) /\ (t2 < S tc1 -> t1 < S tp1)) by (apply (fifo cp m (S tc1) (S tp1) recvmPMTp1 sendmCMTc1 k); crush).
-        destruct big as [useful junk]; clear junk.
-        assert (lt1: tc1 < S tp1) by crush.
-        assert (lt2: t1 < S tp1) by crush.
-        clear lt1.
-        specialize (useful lt2).
-        crush.
-
-        assert (hyp2: forall k t1 t2, recvm c k t1 -> sendm p k t2 -> t1 <= tc1 -> t2 <= tp2).
-        intros.
-        assert (big: (t1 < S tc2 -> t2 < S tp2) /\ (t2 < S tp2 -> t1 < S tc2)) by (apply (fifo pc n (S tp2) (S tc2) cRecvN pSendN k); crush).
-        destruct big as [useful junk]; clear junk.
-        assert (lt1: tc1 < S tc2) by crush.
-        assert (lt2: t1 < S tc2) by crush.
-        clear lt1.
-        specialize (useful lt2).
-        crush.
-
-        assert (basic: tp2 < tpmin) by crush.
-
-        clear tp1LeTpmin m recvmPMTp1 noRecvGTTp1 tc1LeTp1 sendmCMTc1 tc1LeTcmin tc1LtTc2LeTcmin exCRecv n cRecvN fstN tp2LeTc2 pSendN tc1LeTc2 noCRecv tp2LtTp1.
-
-        clear tp1 tc2.
-
-        assert (exists x y, x < tpmin /\ (forall m t1 t2, recvm p m t1 -> sendm c m t2 -> t1 <= x -> t2 <= y) /\ (forall m t1 t2, recvm c m t1 -> sendm p m t2 -> t1 <= y -> t2 <= x) /\ nextState c y > nextState p x) by (exists tp2; exists tc1; crush).
-
-        crush.
-      Qed.
-
-      Theorem conservative'':
-        forall t, ~ (nextState c t > nextState p t).
-      Proof.
-        intro t.
-        apply strongLess.
-        intro.
-        intro.
-        intro.
-        intro recv.
-        intro send.
-        intro le.
-        pose proof (deqImpEnq cp m t1 recv) as exEnq.
-        destruct exEnq as [t' rest].
-        destruct rest as [le2 enq].
-        pose proof (uniqueEnq cp m m t2 t' send enq).
-        destruct H as [useful junk].
-        crush.
-        intro.
-        intro.
-        intro.
-        intro recv.
-        intro send.
-        intro le.
-        pose proof (deqImpEnq pc m t1 recv) as exEnq.
-        destruct exEnq as [t' rest].
-        destruct rest as [le2 enq].
-        pose proof (uniqueEnq pc m m t2 t' send enq).
-        destruct H as [useful junk].
-        crush.
-      Qed.
-
-      Theorem conservative':
-        forall t, ~ state c t > state p t.
-      Proof.
-        intro.
-        destruct t.
-        unfold not; crush.
-        apply (conservative'' t).
-      Qed.
-
-      Theorem conservative:
-        forall t, state c t <= state p t.
-      Proof.
-        intro.
-        pose proof (conservative' t).
-        crush.
-      Qed.
-    End message.
-  End fifo.
-End classic.
-
-Check conservative.
+  Theorem conservative t:
+    state c t <= state p t.
+  Proof.
+    pose proof (conservative' t).
+    crush.
+  Qed.
+End Resp.
